this might work

Impl/BookkeepingImpl.i.dfy
@@ -1,11 +1,11 @@
 include "IOImpl.i.dfy"
-// include "BookkeepingModel.i.dfy"
+include "BookkeepingModel.i.dfy"
 
 module BookkeepingImpl { 
   import opened IOImpl
   import opened StateBCImpl
   import opened DiskOpImpl
-  // import BookkeepingModel
+  import BookkeepingModel
   import LruModel
 
   import opened Options
@@ -17,11 +17,7 @@ module BookkeepingImpl {
   import IndirectionTable
 
   import opened Bounds
-  import opened NodeImpl
 
-  import SSM = StateSectorModel
-
-  // TODO(andreal) dedup with the definition in the model
   predicate RefAvailable(s: ImplVariables, ref: Reference)
     requires s.Ready? && s.W()
   {
@@ -54,7 +50,6 @@ module BookkeepingImpl {
     {
       var cacheLookup := s.cache.InCache(i);
       if !cacheLookup {
-        // assert RefAvailable(s, i);
         return Some(i);
       }
       
@@ -71,8 +66,6 @@ module BookkeepingImpl {
   requires s.Ready?
   requires s.W()
 
-  ensures s.Ready?
-  ensures s.W()
   ensures ref.Some? ==> ref.value != avoid;
   ensures ref.Some? ==> RefAvailable(s, ref.value)
   ensures forall ref1 | ref1 in s.cache.I() :: Some(ref1) != ref
@@ -104,37 +97,9 @@ module BookkeepingImpl {
     }
   }
 
-  // Conditions that will hold intermediately between writes and allocs
-  predicate WriteAllocConditions(s: ImplVariables)
-  {
-    && s.Ready?
-    && s.blockAllocator.Inv()
-    && s.ephemeralIndirectionTable.Inv()
-    && s.ephemeralIndirectionTable.TrackingGarbage()
-    && (forall loc |
-        loc in s.ephemeralIndirectionTable.I().locs.Values :: 
-          DiskLayout.ValidNodeLocation(loc))
-    && ConsistentBitmap(s.ephemeralIndirectionTable.I(), s.frozenIndirectionTable.Map((x: IT.IndirectionTable) => x.I()),
-        s.persistentIndirectionTable.I(), s.outstandingBlockWrites, s.blockAllocator.I())
-    && BlockAllocatorModel.Inv(s.blockAllocator.I())
-    && BC.AllLocationsForDifferentRefsDontOverlap(
-        s.ephemeralIndirectionTable.I())
-  }
-
-  predicate ChildrenConditions(s: ImplVariables, succs: Option<seq<BT.G.Reference>>)
-  requires s.Ready?
-  requires s.W()
-  {
-    succs.Some? ==> (
-      && |succs.value| <= MaxNumChildren()
-      && IT.IndirectionTable.SuccsValid(succs.value, s.ephemeralIndirectionTable.graph)
-    )
-  }
-
-  // TODO rewrite in terms of the lemma in BookkeepingModel?
   lemma lemmaIndirectionTableLocIndexValid(s: ImplVariables, ref: BT.G.Reference)
   requires s.W()
-  requires WriteAllocConditions(s)
+  requires s.WriteAllocConditions()
   ensures ref in s.ephemeralIndirectionTable.locs ==>
     (
       && 0 <= s.ephemeralIndirectionTable.locs[ref].addr as int / NodeBlockSize() < NumBlocks()
@@ -154,170 +119,20 @@ module BookkeepingImpl {
     }
   }
 
-  lemma freeIndirectionTableLocCorrect(
-      s: ImplVariables, s': ImplVariables, ref: BT.G.Reference, j: Option<int>)
-  requires WriteAllocConditions(s)
-  requires s'.Ready?
-  requires s'.blockAllocator.Inv()
-  requires forall r | r != ref ::
-      MapsAgreeOnKey(
-          s.ephemeralIndirectionTable.I().locs,
-          s'.ephemeralIndirectionTable.I().locs,
-          r)
-  requires ref !in s'.ephemeralIndirectionTable.I().locs
-  requires j.Some? ==> 0 <= j.value < NumBlocks()
-  requires j.Some? ==> ref in s.ephemeralIndirectionTable.I().locs
-  requires j.Some? ==> s.ephemeralIndirectionTable.I().locs[ref].addr as int == j.value * NodeBlockSize()
-  requires j.Some? ==> s'.blockAllocator.I() == BlockAllocatorModel.MarkFreeEphemeral(s.blockAllocator.I(), j.value)
-  requires j.None? ==> s'.blockAllocator.I() == s.blockAllocator.I()
-  requires j.None? ==> ref !in s.ephemeralIndirectionTable.I().locs
-  ensures (forall i: int :: IT.IndirectionTable.IsLocAllocIndirectionTable(s'.ephemeralIndirectionTable.I(), i)
-      <==> IT.IndirectionTable.IsLocAllocBitmap(s'.blockAllocator.I().ephemeral, i))
-  ensures BlockAllocatorModel.Inv(s'.blockAllocator.I())
-  ensures BC.AllLocationsForDifferentRefsDontOverlap(
-        s'.ephemeralIndirectionTable.I())
-  ensures (forall loc |
-        loc in s'.ephemeralIndirectionTable.I().locs.Values :: 
-          DiskLayout.ValidNodeLocation(loc))
-  {
-    assume false;
-    // reveal_ConsistentBitmap();
-    // BitmapModel.reveal_IsSet();
-    // BitmapModel.reveal_BitUnset();
-    // lemmaIndirectionTableLocIndexValid(s, ref);
-
-    // forall r1, r2 | r1 in s'.ephemeralIndirectionTable.I().locs && r2 in s'.ephemeralIndirectionTable.I().locs
-    // ensures BC.LocationsForDifferentRefsDontOverlap(s'.ephemeralIndirectionTable.I(), r1, r2)
-    // {
-    //   assert MapsAgreeOnKey( s.ephemeralIndirectionTable.I().locs, s'.ephemeralIndirectionTable.I().locs, r1);
-    //   assert MapsAgreeOnKey( s.ephemeralIndirectionTable.I().locs, s'.ephemeralIndirectionTable.I().locs, r2);
-    // }
-
-    // forall loc | loc in s'.ephemeralIndirectionTable.I().locs.Values
-    // ensures DiskLayout.ValidNodeLocation(loc)
-    // {
-    //   var r :| r in s'.ephemeralIndirectionTable.I().locs && s'.ephemeralIndirectionTable.I().locs[r] == loc;
-    //   assert MapsAgreeOnKey(s.ephemeralIndirectionTable.I().locs, s'.ephemeralIndirectionTable.I().locs, r);
-    // }
-
-    // if j.Some? {
-    //   assert DiskLayout.ValidNodeLocation(s.ephemeralIndirectionTable.I().locs[ref]);
-    //   assert j.value >= MinNodeBlockIndex() by {
-    //     DiskLayout.reveal_ValidNodeAddr();
-    //   }
-    // }
-
-    // forall i: int
-    // | IT.IndirectionTable.IsLocAllocIndirectionTable(s'.ephemeralIndirectionTable.I(), i)
-    // ensures IT.IndirectionTable.IsLocAllocBitmap(s'.blockAllocator.ephemeral, i)
-    // {
-    //   if j.Some? && i == j.value {
-    //     if 0 <= i < MinNodeBlockIndex() {
-    //       assert false;
-    //     } else {
-    //       var r :| r in s'.ephemeralIndirectionTable.locs &&
-    //           s'.ephemeralIndirectionTable.locs[r].addr as int == i * NodeBlockSize() as int;
-    //       assert MapsAgreeOnKey(
-    //         s.ephemeralIndirectionTable.I().locs,
-    //         s'.ephemeralIndirectionTable.I().locs, r);
-
-    //       assert BC.LocationsForDifferentRefsDontOverlap(s.ephemeralIndirectionTable.I(), ref, r);
-
-    //       assert ref !in s'.ephemeralIndirectionTable.I().locs;
-    //       assert r in s'.ephemeralIndirectionTable.I().locs;
-    //       assert s.ephemeralIndirectionTable.I().locs[r]
-    //           == s.ephemeralIndirectionTable.I().locs[ref];
-    //       assert r == ref;
-
-    //       assert false;
-    //     }
-    //   } else {
-    //     if 0 <= i < MinNodeBlockIndex() {
-    //       assert IT.IndirectionTable.IsLocAllocIndirectionTable(s.ephemeralIndirectionTable.I(), i);
-    //       assert IT.IndirectionTable.IsLocAllocBitmap(s.blockAllocator.ephemeral, i);
-    //       assert IT.IndirectionTable.IsLocAllocBitmap(s'.blockAllocator.ephemeral, i);
-    //     } else {
-    //       var r :| r in s'.ephemeralIndirectionTable.locs &&
-    //           s'.ephemeralIndirectionTable.locs[r].addr as int == i * NodeBlockSize() as int;
-    //       assert MapsAgreeOnKey(
-    //         s.ephemeralIndirectionTable.I().locs,
-    //         s'.ephemeralIndirectionTable.I().locs, r);
-    //       assert IT.IndirectionTable.IsLocAllocIndirectionTable(s.ephemeralIndirectionTable.I(), i);
-    //       assert IT.IndirectionTable.IsLocAllocBitmap(s.blockAllocator.ephemeral, i);
-    //       assert IT.IndirectionTable.IsLocAllocBitmap(s'.blockAllocator.ephemeral, i);
-    //     }
-    //   }
-    // }
-
-    // forall i: int
-    // | IT.IndirectionTable.IsLocAllocBitmap(s'.blockAllocator.ephemeral, i)
-    // ensures IT.IndirectionTable.IsLocAllocIndirectionTable(s'.ephemeralIndirectionTable.I(), i)
-    // {
-    //   if j.Some? && i == j.value {
-    //     assert IT.IndirectionTable.IsLocAllocIndirectionTable(s'.ephemeralIndirectionTable.I(), i);
-    //   } else {
-    //     assert IT.IndirectionTable.IsLocAllocBitmap(s.blockAllocator.ephemeral, i);
-    //     assert IT.IndirectionTable.IsLocAllocIndirectionTable(s.ephemeralIndirectionTable.I(), i);
-    //     if 0 <= i < MinNodeBlockIndex() {
-    //       assert IT.IndirectionTable.IsLocAllocIndirectionTable(s'.ephemeralIndirectionTable.I(), i);
-    //     } else {
-    //       var r :| r in s.ephemeralIndirectionTable.locs &&
-    //         s.ephemeralIndirectionTable.locs[r].addr as int == i * NodeBlockSize() as int;
-    //       assert MapsAgreeOnKey(
-    //         s.ephemeralIndirectionTable.I().locs,
-    //         s'.ephemeralIndirectionTable.I().locs, r);
-    //       assert r in s'.ephemeralIndirectionTable.locs &&
-    //         s'.ephemeralIndirectionTable.locs[r].addr as int == i * NodeBlockSize() as int;
-    //       assert IT.IndirectionTable.IsLocAllocIndirectionTable(s'.ephemeralIndirectionTable.I(), i);
-    //     }
-    //   }
-    // }
-
-    // if j.Some? {
-    //   forall i | 0 <= i < NumBlocks()
-    //   ensures BitmapModel.IsSet(s'.blockAllocator.full, i) == (
-    //     || BitmapModel.IsSet(s'.blockAllocator.ephemeral, i)
-    //     || (s'.blockAllocator.frozen.Some? && BitmapModel.IsSet(s'.blockAllocator.frozen.value, i))
-    //     || BitmapModel.IsSet(s'.blockAllocator.persistent, i)
-    //     || BitmapModel.IsSet(s'.blockAllocator.full, i)
-    //   )
-    //   {
-    //     if i == j.value {
-    //     } else {
-    //       assert BitmapModel.IsSet(s'.blockAllocator.full, i) == BitmapModel.IsSet(s.blockAllocator.full, i);
-    //       assert BitmapModel.IsSet(s'.blockAllocator.ephemeral, i) == BitmapModel.IsSet(s.blockAllocator.ephemeral, i);
-    //       assert s'.blockAllocator.frozen.Some? ==> BitmapModel.IsSet(s'.blockAllocator.frozen.value, i) == BitmapModel.IsSet(s.blockAllocator.frozen.value, i);
-    //       assert BitmapModel.IsSet(s'.blockAllocator.persistent, i) == BitmapModel.IsSet(s.blockAllocator.persistent, i);
-    //       assert BitmapModel.IsSet(s'.blockAllocator.outstanding, i) == BitmapModel.IsSet(s.blockAllocator.outstanding, i);
-    //     }
-    //   }
-    // } else {
-    // }
-  }
-
   method writeBookkeeping(linear inout s: ImplVariables, ref: BT.G.Reference, children: Option<seq<BT.G.Reference>>)
   requires old_s.W()
   requires old_s.Ready?
   requires |LruModel.I(old_s.lru.Queue())| <= 0x1_0000_0000
-  requires WriteAllocConditions(old_s)
-  requires ChildrenConditions(old_s, children)
+  requires old_s.WriteAllocConditions()
+  requires old_s.ChildrenConditions(children)
   requires |old_s.ephemeralIndirectionTable.I().graph| < IndirectionTable.MaxSize()
 
-  ensures s.Ready?
   ensures s.W()
+  ensures s.Ready?
   ensures |LruModel.I(s.lru.Queue())| <= |LruModel.I(old_s.lru.Queue())| + 1
   ensures s.cache.I() == old_s.cache.I()
-  ensures s.totalCacheSize() == old_s.totalCacheSize();
-  ensures WriteAllocConditions(s)
-  ensures |s.ephemeralIndirectionTable.graph| <= |old_s.ephemeralIndirectionTable.graph| + 1
 
-  ensures forall children1 :: ChildrenConditions(old_s, children1) ==> ChildrenConditions(s, children1)
-  ensures forall childrenValue:: ChildrenConditions(old_s, Some(childrenValue)) ==> (
-        forall i :: 0 <= i < |childrenValue| ==> ChildrenConditions(s, Some(childrenValue[i := ref])))
-  ensures forall ref2 :: ref2 in old_s.ephemeralIndirectionTable.I().graph ==>  ref2 in s.ephemeralIndirectionTable.I().graph
-  ensures ref in s.ephemeralIndirectionTable.I().graph
-  ensures ChildrenConditions(s, Some([ref]))
-  ensures LruModel.I(s.lru.Queue()) == LruModel.I(old_s.lru.Queue()) + {ref}
+  ensures s.IBlockCache2() == BookkeepingModel.writeBookkeeping(old_s.IBlockCache2(), ref, children)
   {
     lemmaIndirectionTableLocIndexValid(s, ref);
     var oldLoc := inout s.ephemeralIndirectionTable.UpdateAndRemoveLoc(ref, (if children.Some? then children.value else []));
@@ -333,30 +148,24 @@ module BookkeepingImpl {
     assert |LruModel.I(s.lru.Queue())| == |LruModel.I(old_s.lru.Queue()) + {ref}|
         <= |LruModel.I(old_s.lru.Queue())| + |{ref}|
         == |LruModel.I(old_s.lru.Queue())| + 1;
-    
-    freeIndirectionTableLocCorrect(old_s, s, ref,
-      if oldLoc.Some?
-      then Some(oldLoc.value.addr as int / NodeBlockSize())
-      else None);
-    reveal_ConsistentBitmap();
+
+    reveal BookkeepingModel.writeBookkeeping(); 
   }
+/*
 
   method writeBookkeepingNoSuccsUpdate(linear inout s: ImplVariables, ref: BT.G.Reference)
   requires old_s.W()
   requires old_s.Ready?
-
   requires |LruModel.I(old_s.lru.Queue())| <= 0x1_0000_0000
-  requires WriteAllocConditions(old_s)
+  requires BookkeepingModel.WriteAllocConditions(old_s.I())
   requires ref in old_s.ephemeralIndirectionTable.I().graph
-
   ensures s.W()
-  ensures s.Ready?
+  ensures s.I() == BookkeepingModel.writeBookkeepingNoSuccsUpdate(old_s.I(), ref)
   ensures |LruModel.I(s.lru.Queue())| <= |LruModel.I(old_s.lru.Queue())| + 1
-  ensures WriteAllocConditions(s)
-  ensures |s.ephemeralIndirectionTable.graph| <= |old_s.ephemeralIndirectionTable.graph| + 1
-  // [yizhou7] post condition probably not strong enough
   {
-    lemmaIndirectionTableLocIndexValid(s, ref);
+    BookkeepingModel.reveal_writeBookkeepingNoSuccsUpdate();
+
+    BookkeepingModel.lemmaIndirectionTableLocIndexValid(s.I(), ref);
 
     var oldLoc := inout s.ephemeralIndirectionTable.RemoveLoc(ref);
 
@@ -371,12 +180,6 @@ module BookkeepingImpl {
     assert |LruModel.I(s.lru.Queue())| == |LruModel.I(old_s.lru.Queue()) + {ref}|
         <= |LruModel.I(old_s.lru.Queue())| + |{ref}|
         == |LruModel.I(old_s.lru.Queue())| + 1;
-
-    freeIndirectionTableLocCorrect(old_s, s, ref,
-      if oldLoc.Some?
-      then Some(oldLoc.value.addr as int / NodeBlockSize())
-      else None);
-    reveal_ConsistentBitmap();
   }
 
   method allocBookkeeping(linear inout s: ImplVariables, children: Option<seq<BT.G.Reference>>)
@@ -384,102 +187,21 @@ module BookkeepingImpl {
   requires old_s.W()
   requires old_s.Ready?
   requires |LruModel.I(old_s.lru.Queue())| <= 0x1_0000_0000
-  requires WriteAllocConditions(old_s)
-  requires ChildrenConditions(old_s, children)
+  requires BookkeepingModel.WriteAllocConditions(old_s.I())
+  requires BookkeepingModel.ChildrenConditions(old_s.I(), children)
   requires |old_s.ephemeralIndirectionTable.I().graph| < IndirectionTable.MaxSize()
   ensures s.Ready?
   ensures s.W()
+  ensures (s.I(), ref) == BookkeepingModel.allocBookkeeping(old_s.I(), children)
   ensures |LruModel.I(s.lru.Queue())| <= |LruModel.I(old_s.lru.Queue())| + 1
   ensures s.cache.I() == old_s.cache.I()
-  ensures s.totalCacheSize() == old_s.totalCacheSize();
-  ensures WriteAllocConditions(s)
-  ensures |s.ephemeralIndirectionTable.graph| <= |old_s.ephemeralIndirectionTable.graph| + 1
-  ensures ref.Some? ==> ChildrenConditions(s, Some([ref.value]))
-  ensures ref.Some? ==> (forall ref2 :: ref2 in old_s.cache.I() ==> ref.value != ref2)
-  ensures ref.Some? ==> (ref.value !in old_s.cache.I())
-  ensures ref.Some? ==> 
-      (
-        forall childrenValue:: ChildrenConditions(old_s, Some(childrenValue)) ==> (
-        forall i :: 0 <= i < |childrenValue| ==> ChildrenConditions(s, Some(childrenValue[i := ref.value])))
-      )
-  ensures ref.Some? ==> (LruModel.I(s.lru.Queue()) == LruModel.I(old_s.lru.Queue()) + {ref.value})
-  ensures ref.None? ==> old_s == s;
   {
+    BookkeepingModel.reveal_allocBookkeeping();
+    
     ref := getFreeRef(s);
-    if ref.Some? {
+    if (ref.Some?) {
       writeBookkeeping(inout s, ref.value, children);
     }
   }
-
-  lemma lemmaChildrenConditionsOfNode(
-      s: ImplVariables, ref: BT.G.Reference)
-  requires s.Ready?
-  requires s.BCInv()
-  requires ref in s.cache.I()
-  requires ref in s.ephemeralIndirectionTable.graph
-  ensures ChildrenConditions(s, s.cache.I()[ref].children)
-  // {
-  //   if s.cache[ref].children.Some? {
-  //     forall r | r in s.cache[ref].children.value
-  //     ensures r in s.ephemeralIndirectionTable.graph
-  //     {
-  //       // Trigger the forall in CacheConsistentWithSuccessors
-  //       assert r in BT.G.Successors(INode(s.cache[ref]));
-  //       assert r in s.ephemeralIndirectionTable.graph[ref];
-  //     }
-  //   }
-  // }
-
-  // method writeWithNode(linear inout s: ImplVariables, ref: BT.G.Reference, linear node: Node)
-  // requires old_s.WFBCVars()
-  // requires old_s.Ready?
-  // requires old_s.totalCacheSize() <= MaxCacheSize()
-  
-  // requires WriteAllocConditions(old_s)
-  // requires ChildrenConditions(old_s, node.children)
-  // requires |old_s.ephemeralIndirectionTable.graph| < IT.MaxSize()
-  // requires |LruModel.I(old_s.lru.Queue())| <= 0x1_0000_0000
-  // requires node.Inv()
-  // requires SSM.WFNode(node.I())
-
-  // requires ref in old_s.ephemeralIndirectionTable.I().graph
-  // requires ref in old_s.cache.I()
-
-  // requires BC.BlockPointsToValidReferences(node.I(), old_s.ephemeralIndirectionTable.I().graph)
-  // requires old_s.frozenIndirectionTable.lSome? && ref in old_s.frozenIndirectionTable.value.graph ==> ref in old_s.frozenIndirectionTable.value.locs
-
-  // ensures s.WFBCVars()
-  // ensures s.Ready?
-
-  // ensures BC.Dirty(old_s.IBlockCache(), s.IBlockCache(), ref, node.I())
-  // ensures old_s.TotalCacheSize() == s.TotalCacheSize()
-
-  // ensures WriteAllocConditions(s)
-  // ensures |s.ephemeralIndirectionTable.graph| <= |old_s.ephemeralIndirectionTable.graph| + 1
-  // {
-  //   lemmaIndirectionTableLocIndexValid(s, ref);
-  //   var oldLoc := inout s.ephemeralIndirectionTable.UpdateAndRemoveLoc(ref, (if node.children.Some? then node.children.value else []));
-
-  //   inout s.lru.Use(ref);
-
-  //   if oldLoc.Some? {
-  //     inout s.blockAllocator.MarkFreeEphemeral(oldLoc.value.addr / NodeBlockSizeUint64());
-  //   }
-
-  //   inout s.cache.Insert(ref, node);
-
-  //   LruModel.LruUse(old_s.lru.Queue(), ref);
-  //   assert LruModel.I(s.lru.Queue()) == LruModel.I(old_s.lru.Queue()) + {ref};
-  //   assert |LruModel.I(s.lru.Queue())| == |LruModel.I(old_s.lru.Queue()) + {ref}|
-  //       <= |LruModel.I(old_s.lru.Queue())| + |{ref}|
-  //       == |LruModel.I(old_s.lru.Queue())| + 1;
-    
-  //   freeIndirectionTableLocCorrect(old_s, s, ref,
-  //     if oldLoc.Some?
-  //     then Some(oldLoc.value.addr as int / NodeBlockSize())
-  //     else None);
-  //   reveal_ConsistentBitmap();
-
-  //   assert s.WFBCVars();
-  // }
+  */
 }
