Impl/BookkeepingModel.i.dfy
@@ -17,95 +17,114 @@ module BookkeepingModel {
   import opened Bounds
   import LruModel
   import DiskLayout
-  import BBC = BetreeCache
 
   import opened NativeTypes
 
   predicate RefAvailable(s: BBC.Variables, ref: Reference)
-    requires s.Ready?
   {
+    && s.Ready?
     && ref !in s.ephemeralIndirectionTable.graph
-    && ref !in s.cache
+    && ref !in s.cache 
     && ref != BT.G.Root()
   }
 
-  // fullWrite and fullAlloc are like writeBookkeeping/allocBookkeeping, except that fullWrite and fullAlloc update
-  // the cache with the node. In the implementation of betree operations we use the above,
-  // because it turns out to be easier to do the cache updates separately. However, for the proofs
-  // it is easier to use the below.
+  // function getFreeRefIterate(s: BBC.Variables, i: uint64) 
+  // : (ref : Option<BT.G.Reference>)
+  // requires s.Ready?
+  // // requires s.ephemeralIndirectionTable.Inv()
+  // requires i >= 1
+  // requires forall r | r in s.ephemeralIndirectionTable.graph :: r < i
+  // ensures ref.Some? ==> RefAvailable(s, ref.value)
+  // decreases 0x1_0000_0000_0000_0000 - i as int
+  // {
+  //   // NOTE: we shouldn't even need to do this check with the current
+  //   // setup (because we start i at a value > than anything that has
+  //   // *ever* been in the ephemeralIndirectionTable, which would include
+  //   // anything in the cache. That requires some proof though.
+  //   if i !in s.cache then (
+  //     Some(i)
+  //   ) else if i == 0xffff_ffff_ffff_ffff then (
+  //     None
+  //   ) else (
+  //     getFreeRefIterate(s, i+1) 
+  //   )
+  // }
 
-  function writeWithNode(s: BBC.Variables, ref: BT.G.Reference, node: Node)
-  : (s': BBC.Variables)
-    requires s.WriteAllocConditions()
-    ensures s'.WriteAllocConditions()
-    ensures |s'.ephemeralIndirectionTable.graph| <= |s.ephemeralIndirectionTable.graph| + 1
+  // function {:opaque} getFreeRef(s: BBC.Variables)
+  // : (ref : Option<BT.G.Reference>)
+  // requires s.Ready?
+  // // requires s.ephemeralIndirectionTable.Inv()
+  // ensures ref.Some? ==> RefAvailable(s, ref.value)
+  // {
+  //   var i := s.ephemeralIndirectionTable.getRefUpperBound();
+  //   if i == 0xffff_ffff_ffff_ffff then (
+  //     None
+  //   ) else (
+  //     getFreeRefIterate(s, i+1)
+  //   )
+  // }
+
+  // function getFreeRef2Iterate(s: BBC.Variables, avoid: BT.G.Reference, i: uint64) 
+  // : (ref : Option<BT.G.Reference>)
+  // requires s.Ready?
+  // // requires s.ephemeralIndirectionTable.Inv()
+  // requires i >= 1
+  // requires forall r | r in s.ephemeralIndirectionTable.graph :: r < i
+  // ensures ref.Some? ==> RefAvailable(s, ref.value)
+  // ensures ref.Some? ==> ref.value != avoid
+  // decreases 0x1_0000_0000_0000_0000 - i as int
+  // {
+  //   if i != avoid && i !in s.cache then (
+  //     Some(i)
+  //   ) else if i == 0xffff_ffff_ffff_ffff then (
+  //     None
+  //   ) else (
+  //     getFreeRef2Iterate(s, avoid, i+1) 
+  //   )
+  // }
+
+  // function {:opaque} getFreeRef2(s: BBC.Variables, avoid: BT.G.Reference)
+  // : (ref : Option<BT.G.Reference>)
+  // requires s.Ready?
+  // // requires s.ephemeralIndirectionTable.Inv()
+  // ensures ref.Some? ==> RefAvailable(s, ref.value)
+  // ensures ref.Some? ==> ref.value != avoid
+  // {
+  //   var i := s.ephemeralIndirectionTable.getRefUpperBound();
+  //   if i == 0xffff_ffff_ffff_ffff then (
+  //     None
+  //   ) else (
+  //     getFreeRef2Iterate(s, avoid, i+1)
+  //   )
+  // }
+
+  // Conditions that will hold intermediately between writes and allocs
+  predicate WriteAllocConditions(s: BBC.Variables)
   {
-    var succs := if node.children.Some? then node.children.value else [];
-    var oldLoc := MapLookupOption(s.ephemeralIndirectionTable.locs, ref);
-    // TODO(andreal) s.ephemeralIndirectionTable.updateAndRemoveLoc(ref,
-    // TODO(andreal)     (if node.children.Some? then node.children.value else []));
-    var eph := s.ephemeralIndirectionTable.(
-      graph := s.ephemeralIndirectionTable.graph[ref := succs]).(
-      locs := MapRemove1(s.ephemeralIndirectionTable.locs, ref));
-    var s' := s.(ephemeralIndirectionTable := eph).(cache := s.cache[ref := node]);
-    assert s'.WriteAllocConditions();
-    s'
+    && s.Ready?
+    && (forall loc | loc in s.ephemeralIndirectionTable.locs.Values :: 
+          DiskLayout.ValidNodeLocation(loc))
+    && BC.AllLocationsForDifferentRefsDontOverlap(s.ephemeralIndirectionTable)
   }
 
-  lemma writeCorrect(s: BBC.Variables, ref: BT.G.Reference, node: Node)
-  requires s.WriteAllocConditions()
-  requires ref in s.ephemeralIndirectionTable.graph
-  requires ref in s.cache
-  // requires WFNode(node)
-  requires BC.BlockPointsToValidReferences(INode(node), s.ephemeralIndirectionTable.graph)
-  requires s.frozenIndirectionTable.Some? && ref in s.frozenIndirectionTable.value.graph ==> ref in s.frozenIndirectionTable.value.locs
-  // requires |s.ephemeralIndirectionTable.graph| < IT.MaxSize()
-  ensures var s' := writeWithNode(s, ref, node);
-    && BC.Dirty(s, s', ref, INode(node))
-    && s'.totalCacheSize() == s.totalCacheSize()
-    && s'.WriteAllocConditions()
+  predicate ChildrenConditions(s: BBC.Variables, succs: Option<seq<BT.G.Reference>>)
+  requires s.Ready?
   {
-    lemmaIndirectionTableLocIndexValid(s, ref);
-  }
-
-  function allocWithNode(s: BBC.Variables, node: Node)
-  : (p: (BBC.Variables, Option<Reference>))
-  requires s.WriteAllocConditions()
-  requires BC.WFIndirectionTable(s.ephemeralIndirectionTable)
-  requires BC.BlockPointsToValidReferences(INode(node), s.ephemeralIndirectionTable.graph)
-  ensures var (s', ref) := p;
-    && s'.WriteAllocConditions()
-    && |s'.ephemeralIndirectionTable.graph| <= |s.ephemeralIndirectionTable.graph| + 1
-    && (ref.Some? ==> BC.Alloc(s, s', ref.value, INode(node)))
-    && (ref.None? ==> s' == s)
-    && (ref.Some? ==> s'.totalCacheSize() == s.totalCacheSize() + 1)
-    && s'.WriteAllocConditions()
-  {
-    var ref: Option<BT.G.Reference> :| ref.Some? ==> RefAvailable(s, ref.value);
-    if ref.Some? then (
-      lemmaIndirectionTableLocIndexValid(s, ref.value);
-      var s' := writeWithNode(s, ref.value, node);
-      assert ref.value !in s.ephemeralIndirectionTable.locs;
-      assert s'.ephemeralIndirectionTable.locs == s.ephemeralIndirectionTable.locs;
-      assert BC.Alloc(s, s', ref.value, INode(node));
-      (s', ref)
-    ) else (
-      (s, None)
+    succs.Some? ==> (
+      && |succs.value| <= MaxNumChildren()
+      && IT.IndirectionTable.SuccsValid(succs.value, s.ephemeralIndirectionTable.graph)
     )
   }
 
-  // lemma allocCorrect(s: BBC.Variables, node: Node) //merged
-
   lemma lemmaIndirectionTableLocIndexValid(s: BBC.Variables, ref: BT.G.Reference)
-  requires s.WriteAllocConditions()
+  requires WriteAllocConditions(s)
   ensures ref in s.ephemeralIndirectionTable.locs ==>
     (
-      // TODO needed? && 0 <= s.ephemeralIndirectionTable.locs[ref].addr as int / NodeBlockSize() < NumBlocks()
+      // && 0 <= s.ephemeralIndirectionTable.locs[ref].addr as int / NodeBlockSize() < NumBlocks()
       && (s.ephemeralIndirectionTable.locs[ref].addr as int / NodeBlockSize()) * NodeBlockSize() == s.ephemeralIndirectionTable.locs[ref].addr as int
     )
   {
     if ref in s.ephemeralIndirectionTable.locs {
-      reveal_ConsistentBitmap();
       var loc := s.ephemeralIndirectionTable.locs[ref];
       var i := loc.addr as int / NodeBlockSize();
       assert s.ephemeralIndirectionTable.locs[ref] == loc;
@@ -113,37 +132,346 @@ module BookkeepingModel {
       assert DiskLayout.ValidNodeLocation(loc);
       DiskLayout.reveal_ValidNodeAddr();
       assert i * NodeBlockSize() == loc.addr as int;
-      // TODO needed? assert 0 <= s.ephemeralIndirectionTable.locs[ref].addr as int / NodeBlockSize() < NumBlocks();
     }
   }
 
-  lemma lemmaChildInGraph(s: BBC.Variables, ref: BT.G.Reference, childref: BT.G.Reference)
-  requires s.Ready?
-  requires BBC.Inv(s)
-  requires ref in s.cache
-  requires ref in s.ephemeralIndirectionTable.graph
-  requires childref in BT.G.Successors(INode(s.cache[ref]))
-  ensures childref in s.ephemeralIndirectionTable.graph
-  {
-    assert childref in s.ephemeralIndirectionTable.graph[ref];
-  }
+  // Bookkeeping only - we update the cache with the Node separately.
+  // This turns out to be easier to do.
 
-  lemma lemmaBlockPointsToValidReferences(s: BBC.Variables, ref: BT.G.Reference)
-  requires s.Ready?
-  requires BBC.Inv(s)
-  requires ref in s.cache
-  requires ref in s.ephemeralIndirectionTable.graph
-  ensures BC.BlockPointsToValidReferences(INode(s.cache[ref]), s.ephemeralIndirectionTable.graph);
+  function {:opaque} writeBookkeeping(s: BBC.Variables, ref: BT.G.Reference, children: Option<seq<BT.G.Reference>>)
+  : (s': BBC.Variables)
+  requires WriteAllocConditions(s)
+  requires ChildrenConditions(s, children)
+  // requires |s.ephemeralIndirectionTable.graph| < IT.MaxSize()
+  ensures s'.Ready?
+  ensures s'.cache == s.cache
+  ensures WriteAllocConditions(s')
+  ensures |s'.ephemeralIndirectionTable.graph| <= |s.ephemeralIndirectionTable.graph| + 1
   {
-    var node := INode(s.cache[ref]);
-    var graph := s.ephemeralIndirectionTable.graph;
-    forall r | r in BT.G.Successors(node) ensures r in graph
-    {
-      lemmaChildInGraph(s, ref, r);
-    }
+    // lemmaIndirectionTableLocIndexValid(s, ref);
+    var succs := if children.Some? then children.value else [];
+    var oldLoc := MapLookupOption(s.ephemeralIndirectionTable.locs, ref);
+    // TODO(andreal) s.ephemeralIndirectionTable.updateAndRemoveLoc(ref,
+    // TODO(andreal)     (if children.Some? then children.value else []));
+    var eph := s.ephemeralIndirectionTable.(
+      graph := s.ephemeralIndirectionTable.graph[ref := succs]).(
+      locs := MapRemove1(s.ephemeralIndirectionTable.locs, ref));
+    var s' := s.(ephemeralIndirectionTable := eph);
+    assert s'.WriteAllocConditions();
+    s'    
   }
-
 /*
+
+  function {:opaque} writeBookkeepingNoSuccsUpdate(s: BCVariables, ref: BT.G.Reference)
+  : (s': BCVariables)
+  requires WriteAllocConditions(s)
+  requires ref in s.ephemeralIndirectionTable.graph
+  ensures s'.Ready?
+  ensures s'.cache == s.cache
+  ensures WriteAllocConditions(s')
+  ensures |s'.ephemeralIndirectionTable.graph| <= |s.ephemeralIndirectionTable.graph| + 1
+  {
+    lemmaIndirectionTableLocIndexValid(s, ref);
+    var (eph, oldLoc) := s.ephemeralIndirectionTable.removeLoc(ref);
+    var blockAllocator' := if oldLoc.Some?
+      then BlockAllocatorModel.MarkFreeEphemeral(s.blockAllocator, oldLoc.value.addr as int / NodeBlockSize())
+      else s.blockAllocator;
+    var s' := s.(ephemeralIndirectionTable := eph)
+     .(lru := LruModel.Use(s.lru, ref))
+     .(blockAllocator := blockAllocator');
+
+    freeIndirectionTableLocCorrect(s, s', ref,
+      if oldLoc.Some?
+      then Some(oldLoc.value.addr as int / NodeBlockSize())
+      else None);
+    reveal_ConsistentBitmap();
+
+    s'
+  }
+
+
+  function {:opaque} allocBookkeeping(s: BCVariables, children: Option<seq<BT.G.Reference>>)
+  : (p: (BCVariables, Option<Reference>))
+  requires WriteAllocConditions(s)
+  requires ChildrenConditions(s, children)
+  requires |s.ephemeralIndirectionTable.graph| < IT.MaxSize()
+
+  ensures var (s', id) := p;
+    && s'.Ready?
+    && WriteAllocConditions(s')
+    && |s'.ephemeralIndirectionTable.graph| <= |s.ephemeralIndirectionTable.graph| + 1
+  {
+    var ref := getFreeRef(s);
+    if ref.Some? then (
+      (writeBookkeeping(s, ref.value, children), ref)
+    ) else (
+      (s, None)
+    )
+  }
+
+  // fullWrite and fullAlloc are like writeBookkeeping/allocBookkeeping, except that fullWrite and fullAlloc update
+  // the cache with the node. In the implementation of betree operations we use the above,
+  // because it turns out to be easier to do the cache updates separately. However, for the proofs
+  // it is easier to use the below.
+
+  function writeWithNode(s: BCVariables, ref: BT.G.Reference, node: Node)
+  : (s': BCVariables)
+  requires WriteAllocConditions(s)
+  requires ChildrenConditions(s, node.children)
+  requires |s.ephemeralIndirectionTable.graph| < IT.MaxSize()
+  ensures WriteAllocConditions(s')
+  ensures |s'.ephemeralIndirectionTable.graph| <= |s.ephemeralIndirectionTable.graph| + 1
+  {
+    lemmaIndirectionTableLocIndexValid(s, ref);
+    var (eph, oldLoc) := s.ephemeralIndirectionTable.updateAndRemoveLoc(ref,
+        (if node.children.Some? then node.children.value else []));
+    var blockAllocator' := if oldLoc.Some?
+      then BlockAllocatorModel.MarkFreeEphemeral(s.blockAllocator, oldLoc.value.addr as int / NodeBlockSize())
+      else s.blockAllocator;
+    var s' := s.(ephemeralIndirectionTable := eph).(cache := s.cache[ref := node])
+        .(lru := LruModel.Use(s.lru, ref))
+        .(blockAllocator := blockAllocator');
+
+    freeIndirectionTableLocCorrect(s, s', ref,
+      if oldLoc.Some?
+      then Some(oldLoc.value.addr as int / NodeBlockSize())
+      else None);
+    reveal_ConsistentBitmap();
+
+    s'
+  }
+
+  function allocWithNode(s: BCVariables, node: Node)
+  : (p: (BCVariables, Option<Reference>))
+  requires WriteAllocConditions(s)
+  requires ChildrenConditions(s, node.children)
+  requires |s.ephemeralIndirectionTable.graph| < IT.MaxSize()
+  ensures var (s', id) := p;
+      && WriteAllocConditions(s')
+      && |s'.ephemeralIndirectionTable.graph| <= |s.ephemeralIndirectionTable.graph| + 1
+  {
+    var ref := getFreeRef(s);
+    if ref.Some? then (
+      (writeWithNode(s, ref.value, node), ref)
+    ) else (
+      (s, None)
+    )
+  }
+
+  lemma freeIndirectionTableLocCorrect(
+      s: BCVariables, s': BCVariables, ref: BT.G.Reference, j: Option<int>)
+  requires WriteAllocConditions(s)
+  requires s'.Ready?
+  requires forall r | r != ref ::
+      MapsAgreeOnKey(
+          s.ephemeralIndirectionTable.I().locs,
+          s'.ephemeralIndirectionTable.I().locs,
+          r)
+  requires ref !in s'.ephemeralIndirectionTable.I().locs
+  requires j.Some? ==> 0 <= j.value < NumBlocks()
+  requires j.Some? ==> ref in s.ephemeralIndirectionTable.I().locs
+  requires j.Some? ==> s.ephemeralIndirectionTable.I().locs[ref].addr as int == j.value * NodeBlockSize()
+  requires j.Some? ==> s'.blockAllocator == BlockAllocatorModel.MarkFreeEphemeral(s.blockAllocator, j.value)
+  requires j.None? ==> s'.blockAllocator == s.blockAllocator
+  requires j.None? ==> ref !in s.ephemeralIndirectionTable.I().locs
+  ensures (forall i: int :: IT.IndirectionTable.IsLocAllocIndirectionTable(s'.ephemeralIndirectionTable.I(), i)
+      <==> IT.IndirectionTable.IsLocAllocBitmap(s'.blockAllocator.ephemeral, i))
+  ensures BlockAllocatorModel.Inv(s'.blockAllocator)
+  ensures BC.AllLocationsForDifferentRefsDontOverlap(
+        s'.ephemeralIndirectionTable.I())
+  ensures (forall loc |
+        loc in s'.ephemeralIndirectionTable.I().locs.Values :: 
+          DiskLayout.ValidNodeLocation(loc))
+  {
+    reveal_ConsistentBitmap();
+    BitmapModel.reveal_IsSet();
+    BitmapModel.reveal_BitUnset();
+    lemmaIndirectionTableLocIndexValid(s, ref);
+
+    forall r1, r2 | r1 in s'.ephemeralIndirectionTable.I().locs && r2 in s'.ephemeralIndirectionTable.I().locs
+    ensures BC.LocationsForDifferentRefsDontOverlap(s'.ephemeralIndirectionTable.I(), r1, r2)
+    {
+      assert MapsAgreeOnKey( s.ephemeralIndirectionTable.I().locs, s'.ephemeralIndirectionTable.I().locs, r1);
+      assert MapsAgreeOnKey( s.ephemeralIndirectionTable.I().locs, s'.ephemeralIndirectionTable.I().locs, r2);
+    }
+
+    forall loc | loc in s'.ephemeralIndirectionTable.I().locs.Values
+    ensures DiskLayout.ValidNodeLocation(loc)
+    {
+      var r :| r in s'.ephemeralIndirectionTable.I().locs && s'.ephemeralIndirectionTable.I().locs[r] == loc;
+      assert MapsAgreeOnKey(s.ephemeralIndirectionTable.I().locs, s'.ephemeralIndirectionTable.I().locs, r);
+    }
+
+    if j.Some? {
+      assert DiskLayout.ValidNodeLocation(s.ephemeralIndirectionTable.I().locs[ref]);
+      assert j.value >= MinNodeBlockIndex() by {
+        DiskLayout.reveal_ValidNodeAddr();
+      }
+    }
+
+    forall i: int
+    | IT.IndirectionTable.IsLocAllocIndirectionTable(s'.ephemeralIndirectionTable.I(), i)
+    ensures IT.IndirectionTable.IsLocAllocBitmap(s'.blockAllocator.ephemeral, i)
+    {
+      if j.Some? && i == j.value {
+        if 0 <= i < MinNodeBlockIndex() {
+          assert false;
+        } else {
+          var r :| r in s'.ephemeralIndirectionTable.locs &&
+              s'.ephemeralIndirectionTable.locs[r].addr as int == i * NodeBlockSize() as int;
+          assert MapsAgreeOnKey(
+            s.ephemeralIndirectionTable.I().locs,
+            s'.ephemeralIndirectionTable.I().locs, r);
+
+          assert BC.LocationsForDifferentRefsDontOverlap(s.ephemeralIndirectionTable.I(), ref, r);
+
+          assert ref !in s'.ephemeralIndirectionTable.I().locs;
+          assert r in s'.ephemeralIndirectionTable.I().locs;
+          assert s.ephemeralIndirectionTable.I().locs[r]
+              == s.ephemeralIndirectionTable.I().locs[ref];
+          assert r == ref;
+
+          assert false;
+        }
+      } else {
+        if 0 <= i < MinNodeBlockIndex() {
+          assert IT.IndirectionTable.IsLocAllocIndirectionTable(s.ephemeralIndirectionTable.I(), i);
+          assert IT.IndirectionTable.IsLocAllocBitmap(s.blockAllocator.ephemeral, i);
+          assert IT.IndirectionTable.IsLocAllocBitmap(s'.blockAllocator.ephemeral, i);
+        } else {
+          var r :| r in s'.ephemeralIndirectionTable.locs &&
+              s'.ephemeralIndirectionTable.locs[r].addr as int == i * NodeBlockSize() as int;
+          assert MapsAgreeOnKey(
+            s.ephemeralIndirectionTable.I().locs,
+            s'.ephemeralIndirectionTable.I().locs, r);
+          assert IT.IndirectionTable.IsLocAllocIndirectionTable(s.ephemeralIndirectionTable.I(), i);
+          assert IT.IndirectionTable.IsLocAllocBitmap(s.blockAllocator.ephemeral, i);
+          assert IT.IndirectionTable.IsLocAllocBitmap(s'.blockAllocator.ephemeral, i);
+        }
+      }
+    }
+
+    forall i: int
+    | IT.IndirectionTable.IsLocAllocBitmap(s'.blockAllocator.ephemeral, i)
+    ensures IT.IndirectionTable.IsLocAllocIndirectionTable(s'.ephemeralIndirectionTable.I(), i)
+    {
+      if j.Some? && i == j.value {
+        assert IT.IndirectionTable.IsLocAllocIndirectionTable(s'.ephemeralIndirectionTable.I(), i);
+      } else {
+        assert IT.IndirectionTable.IsLocAllocBitmap(s.blockAllocator.ephemeral, i);
+        assert IT.IndirectionTable.IsLocAllocIndirectionTable(s.ephemeralIndirectionTable.I(), i);
+        if 0 <= i < MinNodeBlockIndex() {
+          assert IT.IndirectionTable.IsLocAllocIndirectionTable(s'.ephemeralIndirectionTable.I(), i);
+        } else {
+          var r :| r in s.ephemeralIndirectionTable.locs &&
+            s.ephemeralIndirectionTable.locs[r].addr as int == i * NodeBlockSize() as int;
+          assert MapsAgreeOnKey(
+            s.ephemeralIndirectionTable.I().locs,
+            s'.ephemeralIndirectionTable.I().locs, r);
+          assert r in s'.ephemeralIndirectionTable.locs &&
+            s'.ephemeralIndirectionTable.locs[r].addr as int == i * NodeBlockSize() as int;
+          assert IT.IndirectionTable.IsLocAllocIndirectionTable(s'.ephemeralIndirectionTable.I(), i);
+        }
+      }
+    }
+
+    if j.Some? {
+      forall i | 0 <= i < NumBlocks()
+      ensures BitmapModel.IsSet(s'.blockAllocator.full, i) == (
+        || BitmapModel.IsSet(s'.blockAllocator.ephemeral, i)
+        || (s'.blockAllocator.frozen.Some? && BitmapModel.IsSet(s'.blockAllocator.frozen.value, i))
+        || BitmapModel.IsSet(s'.blockAllocator.persistent, i)
+        || BitmapModel.IsSet(s'.blockAllocator.full, i)
+      )
+      {
+        if i == j.value {
+        } else {
+          assert BitmapModel.IsSet(s'.blockAllocator.full, i) == BitmapModel.IsSet(s.blockAllocator.full, i);
+          assert BitmapModel.IsSet(s'.blockAllocator.ephemeral, i) == BitmapModel.IsSet(s.blockAllocator.ephemeral, i);
+          assert s'.blockAllocator.frozen.Some? ==> BitmapModel.IsSet(s'.blockAllocator.frozen.value, i) == BitmapModel.IsSet(s.blockAllocator.frozen.value, i);
+          assert BitmapModel.IsSet(s'.blockAllocator.persistent, i) == BitmapModel.IsSet(s.blockAllocator.persistent, i);
+          assert BitmapModel.IsSet(s'.blockAllocator.outstanding, i) == BitmapModel.IsSet(s.blockAllocator.outstanding, i);
+        }
+      }
+    } else {
+    }
+  }
+
+  lemma writeBookkeepingBitmapCorrect(s: BCVariables, ref: BT.G.Reference, children: Option<seq<BT.G.Reference>>)
+  requires WriteAllocConditions(s)
+  requires ChildrenConditions(s, children)
+  requires |s.ephemeralIndirectionTable.graph| < IT.MaxSize()
+  ensures var s' := writeBookkeeping(s, ref, children);
+    && WriteAllocConditions(s')
+  {
+    /*reveal_writeBookkeeping();
+    var s' := writeBookkeeping(s, ref, children);
+
+    lemmaIndirectionTableLocIndexValid(s, ref);
+    assert s.ephemeralIndirectionTable.count as nat < 0x10000000000000000 / 8;
+    var (eph, oldEntry) := MutableMapModel.InsertAndGetOld(s.ephemeralIndirectionTable, ref,
+        (None, if children.Some? then children.value else []));
+
+    var j := if oldEntry.Some? && oldEntry.value.0.Some? then
+      Some(oldEntry.value.0.value.addr as int / NodeBlockSize())
+    else
+      None;
+    freeIndirectionTableLocCorrect(s, s', ref, j);
+    reveal_ConsistentBitmap();*/
+  }
+
+  lemma allocCorrect(s: BCVariables, node: Node)
+  requires WFBCVars(s)
+  requires WriteAllocConditions(s)
+  requires BC.BlockPointsToValidReferences(INode(node), s.ephemeralIndirectionTable.I().graph)
+  requires TotalCacheSize(s) <= MaxCacheSize() - 1
+  requires WFNode(node)
+  requires |s.ephemeralIndirectionTable.graph| < IT.MaxSize()
+  ensures var (s', ref) := allocWithNode(s, node);
+    && WFBCVars(s')
+    && (ref.Some? ==> BC.Alloc(IBlockCache(s), IBlockCache(s'), ref.value, INode(node)))
+    && (ref.None? ==> s' == s)
+    && (ref.Some? ==> TotalCacheSize(s') == TotalCacheSize(s) + 1)
+    && WriteAllocConditions(s')
+  {
+    var ref := getFreeRef(s);
+    if ref.Some? {
+      lemmaIndirectionTableLocIndexValid(s, ref.value);
+      LruModel.LruUse(s.lru, ref.value);
+      writeBookkeepingBitmapCorrect(s, ref.value, node.children);
+      reveal_writeBookkeeping();
+
+      var s' := writeWithNode(s, ref.value, node);
+    }
+  }
+  
+  lemma writeCorrect(s: BCVariables, ref: BT.G.Reference, node: Node)
+  requires s.Ready?
+  requires WFBCVars(s)
+  requires WriteAllocConditions(s)
+  requires ref in s.ephemeralIndirectionTable.I().graph
+  requires ref in s.cache
+  requires WFNode(node)
+  requires BC.BlockPointsToValidReferences(INode(node), s.ephemeralIndirectionTable.I().graph)
+  requires s.frozenIndirectionTable.Some? && ref in s.frozenIndirectionTable.value.graph ==> ref in s.frozenIndirectionTable.value.locs
+  requires |s.ephemeralIndirectionTable.graph| < IT.MaxSize()
+  ensures var s' := writeWithNode(s, ref, node);
+    && WFBCVars(s')
+    && BC.Dirty(IBlockCache(s), IBlockCache(s'), ref, INode(node))
+    && TotalCacheSize(s') == TotalCacheSize(s)
+    && WriteAllocConditions(s')
+  {
+    lemmaIndirectionTableLocIndexValid(s, ref);
+    WeightBucketEmpty();
+
+    LruModel.LruUse(s.lru, ref);
+
+    writeBookkeepingBitmapCorrect(s, ref, node.children);
+    reveal_writeBookkeeping();
+
+    var s' := writeWithNode(s, ref, node);
+    assert WFBCVars(s');
+  }
  
   lemma writeNewRefIsAlloc(s: BCVariables, ref: BT.G.Reference, node: Node)
   requires s.Ready?
@@ -166,9 +494,100 @@ module BookkeepingModel {
     reveal_writeBookkeeping();
   }
 
+  lemma lemmaChildInGraph(s: BCVariables, ref: BT.G.Reference, childref: BT.G.Reference)
+  requires s.Ready?
+  requires BCInv(s)
+  requires ref in s.cache
+  requires ref in s.ephemeralIndirectionTable.graph
+  requires childref in BT.G.Successors(INode(s.cache[ref]))
+  ensures childref in s.ephemeralIndirectionTable.graph
+  {
+    assert childref in s.ephemeralIndirectionTable.I().graph[ref];
+  }
 
+  lemma lemmaBlockPointsToValidReferences(s: BCVariables, ref: BT.G.Reference)
+  requires BCInv(s)
+  requires s.Ready?
+  requires ref in s.cache
+  requires ref in s.ephemeralIndirectionTable.graph
+  ensures BC.BlockPointsToValidReferences(INode(s.cache[ref]), s.ephemeralIndirectionTable.I().graph);
+  {
+    var node := INode(s.cache[ref]);
+    var graph := s.ephemeralIndirectionTable.I().graph;
+    forall r | r in BT.G.Successors(node) ensures r in graph
+    {
+      lemmaChildInGraph(s, ref, r);
+    }
+  }
 
+  lemma getFreeRefIterateDoesntEqual(s: BCVariables, i: uint64, ref: BT.G.Reference)
+  requires s.Ready?
+  requires ref in s.cache
+  requires i >= 1
+  requires s.ephemeralIndirectionTable.Inv()
+  requires forall r | r in s.ephemeralIndirectionTable.graph :: r < i
+  decreases 0x1_0000_0000_0000_0000 - i as int
+  ensures getFreeRefIterate(s, i) != Some(ref)
+  {
+    if i !in s.cache {
+    } else if i == 0xffff_ffff_ffff_ffff {
+    } else {
+      getFreeRefIterateDoesntEqual(s, i+1, ref);
+    }
+  }
 
+  lemma getFreeRefDoesntEqual(s: BCVariables, ref: BT.G.Reference)
+  requires s.Ready?
+  requires ref in s.cache
+  requires s.ephemeralIndirectionTable.Inv()
+  ensures getFreeRef(s) != Some(ref)
+  {
+    reveal_getFreeRef();
+    var i := s.ephemeralIndirectionTable.getRefUpperBound();
+    if i == 0xffff_ffff_ffff_ffff {
+    } else {
+      getFreeRefIterateDoesntEqual(s, i+1, ref);
+    }
+  }
+
+  lemma getFreeRef2IterateDoesntEqual(s: BCVariables, avoid: BT.G.Reference, i: uint64, ref: BT.G.Reference)
+  requires s.Ready?
+  requires ref in s.cache
+  requires i >= 1
+  requires s.ephemeralIndirectionTable.Inv()
+  requires forall r | r in s.ephemeralIndirectionTable.graph :: r < i
+  ensures getFreeRef2Iterate(s, avoid, i) != Some(ref)
+  decreases 0x1_0000_0000_0000_0000 - i as int
+  {
+    if i != avoid && i !in s.cache {
+    } else if i == 0xffff_ffff_ffff_ffff {
+    } else {
+      getFreeRef2IterateDoesntEqual(s, avoid, i+1, ref);
+    }
+  }
+
+  lemma getFreeRef2DoesntEqual(s: BCVariables, avoid: BT.G.Reference, ref: BT.G.Reference)
+  requires s.Ready?
+  requires ref in s.cache
+  requires s.ephemeralIndirectionTable.Inv()
+  ensures getFreeRef2(s, avoid) != Some(ref)
+  {
+    reveal_getFreeRef2();
+    var i := s.ephemeralIndirectionTable.getRefUpperBound();
+    if i == 0xffff_ffff_ffff_ffff {
+    } else {
+      getFreeRef2IterateDoesntEqual(s, avoid, i+1, ref);
+    }
+  }
+
+  lemma allocRefDoesntEqual(s: BCVariables, children: Option<seq<BT.G.Reference>>, ref: BT.G.Reference)
+  requires allocBookkeeping.requires(s, children);
+  requires ref in s.cache
+  ensures allocBookkeeping(s, children).1 != Some(ref)
+  {
+    reveal_allocBookkeeping();
+    getFreeRefDoesntEqual(s, ref);
+  }
 
   lemma lemmaChildrenConditionsOfNode(
       s: BCVariables, ref: BT.G.Reference)
@@ -189,6 +608,47 @@ module BookkeepingModel {
     }
   }
 
+  lemma lemmaChildrenConditionsSingleOfAllocBookkeeping(
+      s: BCVariables, children: Option<seq<BT.G.Reference>>)
+  requires WriteAllocConditions(s)
+  requires ChildrenConditions(s, children)
+  requires |s.ephemeralIndirectionTable.graph| < IT.MaxSize()
+  ensures var (s1, newref) := allocBookkeeping(s, children);
+    newref.Some? ==> ChildrenConditions(s1, Some([newref.value]))
+  {
+    reveal_allocBookkeeping();
+    reveal_writeBookkeeping();
+    //assert newref.value in s1.ephemeralIndirectionTable.graph;
+  }
+
+  lemma lemmaChildrenConditionsUpdateOfAllocBookkeeping(
+      s: BCVariables, children: Option<seq<BT.G.Reference>>,
+          children1: seq<BT.G.Reference>, i: int)
+  requires WriteAllocConditions(s)
+  requires ChildrenConditions(s, children)
+  requires ChildrenConditions(s, Some(children1))
+  requires |s.ephemeralIndirectionTable.graph| < IT.MaxSize()
+  requires 0 <= i < |children1|
+  ensures var (s1, newref) := allocBookkeeping(s, children);
+    newref.Some? ==> ChildrenConditions(s1, Some(children1[i := newref.value]))
+  {
+    reveal_allocBookkeeping();
+    reveal_writeBookkeeping();
+  }
+
+  lemma lemmaChildrenConditionsPreservedWriteBookkeeping(
+      s: BCVariables, ref: BT.G.Reference, children: Option<seq<BT.G.Reference>>,
+      children1: Option<seq<BT.G.Reference>>)
+  requires WriteAllocConditions(s)
+  requires ChildrenConditions(s, children)
+  requires ChildrenConditions(s, children1)
+  requires |s.ephemeralIndirectionTable.graph| < IT.MaxSize()
+  ensures var s1 := writeBookkeeping(s, ref, children);
+    ChildrenConditions(s1, children1)
+  {
+    reveal_writeBookkeeping();
+  }
+
   lemma lemmaChildrenConditionsOfReplace1With2(
       s: BCVariables,
       children: seq<BT.G.Reference>,
@@ -202,6 +662,27 @@ module BookkeepingModel {
   ensures ChildrenConditions(s, Some(replace1with2(children, a, b, i)))
   {
     reveal_replace1with2();
+  }
+
+  lemma lemmaRefInGraphOfWriteBookkeeping(s: BCVariables, ref: BT.G.Reference, children: Option<seq<BT.G.Reference>>)
+  requires WriteAllocConditions(s)
+  requires ChildrenConditions(s, children)
+  requires |s.ephemeralIndirectionTable.graph| < IT.MaxSize()
+  ensures var s1 := writeBookkeeping(s, ref, children);
+    ref in s1.ephemeralIndirectionTable.graph
+  {
+    reveal_writeBookkeeping();
+  }
+
+  lemma lemmaRefInGraphPreservedWriteBookkeeping(s: BCVariables, ref: BT.G.Reference, children: Option<seq<BT.G.Reference>>, ref2: BT.G.Reference)
+  requires WriteAllocConditions(s)
+  requires ChildrenConditions(s, children)
+  requires |s.ephemeralIndirectionTable.graph| < IT.MaxSize()
+  requires ref2 in s.ephemeralIndirectionTable.graph
+  ensures var s1 := writeBookkeeping(s, ref, children);
+    ref2 in s1.ephemeralIndirectionTable.graph
+  {
+    reveal_writeBookkeeping();
   }
   */
 }
